compiler/backend/proofs/clos_to_bvlProofScript.sml
@@ -977,7 +977,7 @@ val env_rel_IMP_EL =
   LESS_LENGTH_env_rel_IMP |> SPEC_ALL |> UNDISCH
   |> CONJUNCT2 |> DISCH_ALL |> GEN_ALL;
 
-(* TODO: there needs to be a PMATCH version of this for translation *)
+(*
 val extract_name_def = Define `
   extract_name [] = (0,[]) /\
   extract_name (x :: xs) =
@@ -991,6 +991,7 @@ val compile_inc_def = Define `
         clos_to_bvl$compile_prog max_app
           (clos_to_bvl$chain_exps n real_es ++ prog)
     : (num, num # exp) alist`;
+*)
 
 val nth_code_def = Define `
   nth_code t_co 0 = LN /\
@@ -1444,8 +1445,9 @@ Proof
      \\ res_tac \\ fs [] \\ rveq \\ fs []
      \\ rw [] \\ res_tac \\ fs []
      \\ imp_res_tac LIST_REL_LENGTH \\ fs [])
-  \\ Cases_on `?i. op = EqualInt i` THEN1
-    (srw_tac[][closSemTheory.do_app_def] \\ fs [] \\ every_case_tac \\ fs [])
+  \\ Cases_on `?i. op = EqualConst i` THEN1
+    (srw_tac[][closSemTheory.do_app_def] \\ fs [] \\ every_case_tac
+     \\ gvs [bvlSemTheory.do_app_def,v_rel_SIMP])
   \\ Cases_on `op = Install` THEN1 fs[closSemTheory.do_app_def]
   \\ Cases_on `op = Equal` THEN1
    (srw_tac[][closSemTheory.do_app_def,bvlSemTheory.do_app_def,
@@ -1592,6 +1594,7 @@ Proof
     every_case_tac \\ fs[v_rel_SIMP] \\ rw[]
     \\ full_simp_tac(srw_ss())[state_rel_def] >> res_tac >> full_simp_tac(srw_ss())[v_rel_SIMP] >>
     rw[] \\ fs[LIST_REL_EL_EQN])
+  >- cheat
   >- (
     Cases_on`xs`>>full_simp_tac(srw_ss())[v_rel_SIMP]>>
     Cases_on`t`>>full_simp_tac(srw_ss())[v_rel_SIMP]>>
@@ -1650,7 +1653,7 @@ val clos_do_app_case_eqs = closSemTheory.do_app_def |> concl
   |> map (type_of o #2 o TypeBase.dest_case)
   |> Redblackset.fromList Type.compare
   |> Redblackset.listItems
-  |> map (TypeBasePure.case_eq_of o Option.valOf o TypeBase.fetch)
+  |> map (TypeBasePure.case_eq_of o Option.valOf o TypeBase.fetch);
 
 val do_app_err = Q.prove(
   `do_app op xs s1 = Rerr err ∧
@@ -1660,7 +1663,7 @@ val do_app_err = Q.prove(
    ⇒
    ∃e. do_app (compile_op op) ys t1 = Rerr e ∧
        exc_rel (v_rel s1.max_app f t1.refs t1.code) err e`,
-  Cases_on `?i. op = EqualInt i` THEN1
+  Cases_on `?i. op = EqualConst i` THEN1
     (srw_tac[][closSemTheory.do_app_def] \\ fs [] \\ every_case_tac \\ fs []) >>
   Cases_on `?tag. op = ConsExtend tag`
   >- (
@@ -1686,8 +1689,7 @@ val do_app_err = Q.prove(
   \\ spose_not_then strip_assume_tac \\ fs[]
   \\ rpt (pop_assum mp_tac)
   \\ rpt (PURE_CASE_TAC \\ fs []) \\ fs []
-  \\ TRY(rpt strip_tac \\ fs[v_rel_cases] \\ fs[state_rel_def] \\ NO_TAC)
-    );
+  \\ TRY(rpt strip_tac \\ fs[v_rel_cases] \\ fs[state_rel_def] \\ NO_TAC));
 
 (* correctness of implemented primitives *)
 
@@ -3035,7 +3037,7 @@ Proof
     \\ rpt (pairarg_tac \\ fs []) \\ rveq \\ fs []
     \\ imp_res_tac compile_exps_LENGTH \\ fs [MAP2_APPEND]
     \\ qunabbrev_tac `progs` \\ fs [markerTheory.Abbrev_def]
-    \\ fs [quantHeuristicsTheory.LIST_LENGTH_2]
+    \\ fs [LENGTH_EQ_NUM_compute]
     \\ rveq \\ fs []
     \\ fs [chain_exps_def]
     \\ rveq \\ fs []
@@ -6155,9 +6157,9 @@ Proof
 QED
 
 Theorem elist_globals_SND_ncompile_inc[simp]:
-   elist_globals (SND (clos_numberProof$compile_inc x y)) = elist_globals y
+   elist_globals (SND (clos_number$compile_inc x y)) = elist_globals y
 Proof
-  rw[clos_numberProofTheory.compile_inc_def,UNCURRY,op_gbag_def,elist_globals_SND_renumber_code_locs_list]
+  rw[clos_numberTheory.compile_inc_def,UNCURRY,op_gbag_def,elist_globals_SND_renumber_code_locs_list]
 QED
 
 Theorem collect_apps_fv1:
@@ -6239,13 +6241,13 @@ Proof
 QED
 
 Theorem mcompile_inc_uncurry:
-   clos_mtiProof$compile_inc max_app p = ((intro_multi max_app (FST p)),[])
+   clos_mti$compile_inc max_app p = ((intro_multi max_app (FST p)),[])
 Proof
   Cases_on`p` \\ EVAL_TAC
 QED
 
 Theorem kcompile_inc_uncurry:
-   clos_knownProof$compile_inc c g p =
+   clos_known$compile_inc c g p =
      (SND (known (reset_inline_factor c) (FST p) [] g),
       MAP FST (FST (known (reset_inline_factor c) (FST p) [] g)),
       SND p)
@@ -6255,14 +6257,14 @@ Proof
 QED
 
 Theorem acompile_inc_uncurry:
-   clos_annotateProof$compile_inc p =
+   clos_annotate$compile_inc p =
    ((annotate 0 (FST p)), clos_annotate$compile (SND p))
 Proof
-  Cases_on`p` \\ rw[clos_annotateProofTheory.compile_inc_def]
+  Cases_on`p` \\ rw[clos_annotateTheory.compile_inc_def]
 QED
 
 Theorem ccompile_inc_uncurry:
-   clos_callProof$compile_inc g p =
+   clos_call$compile_inc g p =
      (FST(SND (calls (FST p) (g,[]))),
       (FST (calls (FST p) (g,[]))),
       SND(SND (calls (FST p) (g,[]))))
@@ -6280,7 +6282,7 @@ Proof
 QED
 
 Theorem fcompile_inc_uncurry:
-   clos_fvsProof$compile_inc p = (compile (FST p), [])
+   clos_fvs$compile_inc p = (compile (FST p), [])
 Proof
   Cases_on`p` \\ EVAL_TAC
 QED
@@ -6405,27 +6407,27 @@ Proof
 QED
 
 Theorem every_Fn_SOME_ncompile_inc[simp]:
-   every_Fn_SOME (SND (clos_numberProof$compile_inc x y))
+   every_Fn_SOME (SND (clos_number$compile_inc x y))
 Proof
-  rw[clos_numberProofTheory.compile_inc_def, UNCURRY]
+  rw[clos_numberTheory.compile_inc_def, UNCURRY]
   \\ rw[Once every_Fn_SOME_EVERY]
   \\ rw[GSYM every_Fn_SOME_EVERY]
   \\ simp[clos_numberProofTheory.renumber_code_locs_every_Fn_SOME]
 QED
 
 Theorem every_Fn_vs_NONE_ncompile_inc[simp]:
-   every_Fn_vs_NONE (SND (clos_numberProof$compile_inc x y)) ⇔ every_Fn_vs_NONE y
+   every_Fn_vs_NONE (SND (clos_number$compile_inc x y)) ⇔ every_Fn_vs_NONE y
 Proof
-  rw[clos_numberProofTheory.compile_inc_def, UNCURRY]
+  rw[clos_numberTheory.compile_inc_def, UNCURRY]
   \\ rw[Once every_Fn_vs_NONE_EVERY]
   \\ rw[GSYM every_Fn_vs_NONE_EVERY]
   \\ simp[clos_numberProofTheory.renumber_code_locs_every_Fn_vs_NONE]
 QED
 
 Theorem ncompile_inc_code_locs_distinct[simp]:
-   ALL_DISTINCT (code_locs (SND (clos_numberProof$compile_inc x y)))
+   ALL_DISTINCT (code_locs (SND (clos_number$compile_inc x y)))
 Proof
-  rw[clos_numberProofTheory.compile_inc_def, UNCURRY]
+  rw[clos_numberTheory.compile_inc_def, UNCURRY]
   \\ rw[Once code_locs_cons]
   \\ rw[Once code_locs_def]
   \\ rw[Once code_locs_def]
@@ -6433,19 +6435,19 @@ Proof
 QED
 
 Theorem code_locs_FST_letop_compile_inc[simp]:
-   code_locs (FST (clos_letopProof$compile_inc x)) = code_locs (FST x)
+   code_locs (FST (clos_letop$compile_inc x)) = code_locs (FST x)
 Proof
-  Cases_on`x` \\ rw[clos_letopProofTheory.compile_inc_def, clos_letopProofTheory.code_locs_let_op]
+  Cases_on`x` \\ rw[clos_letopTheory.compile_inc_def, clos_letopProofTheory.code_locs_let_op]
 QED
 
 Theorem code_locs_FST_ticks_compile_inc[simp]:
-   code_locs (FST (clos_ticksProof$compile_inc x)) = code_locs (FST x)
+   code_locs (FST (clos_ticks$compile_inc x)) = code_locs (FST x)
 Proof
-  Cases_on`x` \\ rw[clos_ticksProofTheory.compile_inc_def, clos_ticksProofTheory.code_locs_remove_ticks]
+  Cases_on`x` \\ rw[clos_ticksTheory.compile_inc_def, clos_ticksProofTheory.code_locs_remove_ticks]
 QED
 
 Theorem code_locs_FST_SND_kcompile_inc:
-   LIST_TO_BAG (code_locs (FST (SND (clos_knownProof$compile_inc x y z)))) ≤
+   LIST_TO_BAG (code_locs (FST (SND (clos_known$compile_inc x y z)))) ≤
    LIST_TO_BAG (code_locs (FST z))
 Proof
   rw[kcompile_inc_uncurry]
@@ -6455,14 +6457,6 @@ Proof
   \\ simp[]
 QED
 
-val cond_call_compile_inc_def = Define`
-  cond_call_compile_inc do_it = if do_it then clos_callProof$compile_inc
-    else CURRY I`;
-
-val cond_mti_compile_inc_def = Define`
-  cond_mti_compile_inc do_it max_app = if do_it
-    then (clos_mtiProof$compile_inc max_app) else I`;
-
 Theorem every_Fn_vs_NONE_cond_call_compile_inc:
   (every_Fn_vs_NONE (FST y)
     ==> every_Fn_vs_NONE (FST (SND (cond_call_compile_inc do_it x y)))) /\
@@ -6470,7 +6464,7 @@ Theorem every_Fn_vs_NONE_cond_call_compile_inc:
     ==> every_Fn_vs_NONE (MAP (SND o SND) (SND (SND (cond_call_compile_inc do_it x y)))))
 Proof
   Cases_on `y`
-  \\ rw [cond_call_compile_inc_def, clos_callProofTheory.compile_inc_def]
+  \\ rw [clos_callTheory.cond_call_compile_inc_def, clos_callTheory.compile_inc_def]
   \\ (pairarg_tac \\ fs [])
   \\ imp_res_tac clos_callProofTheory.calls_preserves_every_Fn_vs_NONE
   \\ fs []
@@ -6483,7 +6477,7 @@ Theorem every_Fn_SOME_cond_call_compile_inc:
     ==> every_Fn_SOME (MAP (SND o SND) (SND (SND (cond_call_compile_inc do_it x y)))))
 Proof
   Cases_on `y`
-  \\ rw [cond_call_compile_inc_def, clos_callProofTheory.compile_inc_def]
+  \\ rw [clos_callTheory.cond_call_compile_inc_def, clos_callTheory.compile_inc_def]
   \\ (pairarg_tac \\ fs [])
   \\ imp_res_tac clos_callProofTheory.calls_preserves_every_Fn_SOME
   \\ fs []
@@ -6492,10 +6486,10 @@ QED
 val compile_common_inc_def = Define`
   compile_common_inc c cc =
   (pure_cc (cond_mti_compile_inc c.do_mti c.max_app)
-    (state_cc (ignore_table clos_numberProof$compile_inc)
+    (state_cc (ignore_table clos_number$compile_inc)
       (clos_knownProof$known_cc c.known_conf
         (state_cc (cond_call_compile_inc c.do_call)
-          (pure_cc clos_annotateProof$compile_inc cc)))))`;
+          (pure_cc clos_annotate$compile_inc cc)))))`;
 
 val clos_state_cc_def = Define `
   clos_state_cc inc (cc : 'b clos_cc) = (state_cc inc cc : ('a # 'b) clos_cc)`;
@@ -6506,7 +6500,7 @@ Theorem semantics_cond_call_compile_inc:
     clos_call$compile do_call es = (es', g, aux) /\
     code = alist_to_fmap aux /\
     (do_call ==> clos_callProof$syntax_ok es /\
-          is_state_oracle clos_callProof$compile_inc co /\
+          is_state_oracle clos_call$compile_inc co /\
           g = FST (FST (co 0)) /\
           oracle_monotonic (set o code_locs o FST o SND) (<)
               (set (code_locs es)) co /\
@@ -6518,7 +6512,7 @@ Theorem semantics_cond_call_compile_inc:
     semantics ffi max_app FEMPTY co
         (clos_state_cc (cond_call_compile_inc do_call) cc) es
 Proof
-  fs [cond_call_compile_inc_def, clos_state_cc_def]
+  fs [clos_callTheory.cond_call_compile_inc_def, clos_state_cc_def]
   \\ reverse CASE_TAC >- (rw [clos_callTheory.compile_def]
         \\ rveq \\ fs [closPropsTheory.semantics_CURRY_I])
   \\ rw []
@@ -6562,7 +6556,7 @@ Theorem semantics_cond_mti_compile_inc:
 Proof
   rw []
   \\ irule (GEN_ALL clos_mtiProofTheory.semantics_compile)
-  \\ fs [cond_mti_compile_inc_def]
+  \\ fs [clos_mtiTheory.cond_mti_compile_inc_def]
   \\ CASE_TAC
   \\ fs [backendPropsTheory.pure_cc_I, backendPropsTheory.pure_co_I]
 QED
@@ -6583,10 +6577,10 @@ Theorem every_Fn_vs_NONE_known_co:
 Proof
   fs [clos_knownProofTheory.known_co_def]
   \\ CASE_TAC \\ fs [backendPropsTheory.SND_state_co]
-  \\ fs (map expand_tup_def [``clos_letopProof$compile_inc``,
-    ``clos_ticksProof$compile_inc``,
-    ``clos_fvsProof$compile_inc``])
-  \\ fs [clos_knownProofTheory.compile_inc_def]
+  \\ fs (map expand_tup_def [``clos_letop$compile_inc``,
+    ``clos_ticks$compile_inc``,
+    ``clos_fvs$compile_inc``])
+  \\ fs [clos_knownTheory.compile_inc_def]
   \\ fs [ UNCURRY ]
   \\ fs [ clos_knownProofTheory.known_every_Fn_vs_NONE ]
 QED
@@ -6601,10 +6595,10 @@ Theorem every_Fn_SOME_known_co:
 Proof
   fs [clos_knownProofTheory.known_co_def]
   \\ CASE_TAC \\ fs [backendPropsTheory.SND_state_co]
-  \\ fs (map expand_tup_def [``clos_letopProof$compile_inc``,
-    ``clos_ticksProof$compile_inc``,
-    ``clos_fvsProof$compile_inc``])
-  \\ fs [clos_knownProofTheory.compile_inc_def]
+  \\ fs (map expand_tup_def [``clos_letop$compile_inc``,
+    ``clos_ticks$compile_inc``,
+    ``clos_fvs$compile_inc``])
+  \\ fs [clos_knownTheory.compile_inc_def]
   \\ fs [ UNCURRY ]
   \\ fs [ clos_knownProofTheory.known_every_Fn_SOME ]
 QED
@@ -6621,15 +6615,15 @@ val obvious_arith_comm = Q.prove (
   Cases_on `b` \\ fs []);
 
 Theorem SND_SND_known_compile_inc:
-  SND (SND (clos_knownProof$compile_inc conf app es)) = SND es
+  SND (SND (clos_known$compile_inc conf app es)) = SND es
 Proof
   Cases_on `es` \\ EVAL_TAC \\ fs [UNCURRY]
 QED
 
-val fvs_inc = ``clos_fvsProof$compile_inc : clos_prog -> clos_prog``;
+val fvs_inc = ``clos_fvs$compile_inc : clos_prog -> clos_prog``;
 
 Theorem known_state_oracle_globals_approx:
-    is_state_oracle (clos_knownProof$compile_inc cfg')
+    is_state_oracle (clos_known$compile_inc cfg')
         (pure_co ^fvs_inc ∘ co) /\
     FST (FST (co 0)) = spt /\
     known cfg exps [] LN = (k_exps, spt) /\
@@ -6659,7 +6653,7 @@ Proof
         backendPropsTheory.is_state_oracle_k
   \\ fs []
   \\ Cases_on `co k` \\ fs [backendPropsTheory.pure_co_def]
-  \\ fs [clos_knownProofTheory.compile_inc_def, fcompile_inc_uncurry]
+  \\ fs [clos_knownTheory.compile_inc_def, fcompile_inc_uncurry]
   \\ rveq \\ fs []
   \\ fs [clos_fvsTheory.compile_def, kcompile_inc_uncurry]
   \\ ConseqConv.CONSEQ_REWRITE_TAC
@@ -6675,7 +6669,7 @@ Theorem known_co_facts:
     let co2 = clos_knownProof$known_co kc co in
     compile kc exps = (kc',exps') ==>
     (IS_SOME kc ==>
-        is_state_oracle (clos_knownProof$compile_inc (THE kc))
+        is_state_oracle (clos_known$compile_inc (THE kc))
             (pure_co ^fvs_inc ∘ co) /\
         FST (FST (co 0)) = (THE kc').val_approx_spt /\
         every_Fn_vs_NONE exps /\ every_Fn_SOME exps /\
@@ -6709,7 +6703,7 @@ Proof
   \\ drule clos_knownProofTheory.known_code_locs_bag
   \\ disch_then (assume_tac o MATCH_MP containerTheory.LIST_TO_BAG_SUBSET)
   \\ fs [clos_fvsTheory.compile_def]
-  \\ fs [clos_ticksProofTheory.compile_inc_def, clos_letopProofTheory.compile_inc_def]
+  \\ fs [clos_ticksTheory.compile_inc_def, clos_letopTheory.compile_inc_def]
   \\ fs [clos_callProofTheory.syntax_ok_def,
     clos_letopProofTheory.code_locs_let_op,
     clos_ticksProofTheory.code_locs_remove_ticks]
@@ -6743,10 +6737,10 @@ val known_co_facts2 = known_co_facts
   |> map GEN_ALL
 
 Theorem MEM_number_compile_inc_locs:
-    MEM x (code_locs (SND (clos_numberProof$compile_inc n exps))) ==>
-    n < x /\ x < FST (clos_numberProof$compile_inc n exps)
+    MEM x (code_locs (SND (clos_number$compile_inc n exps))) ==>
+    n < x /\ x < FST (clos_number$compile_inc n exps)
 Proof
-  fs [clos_numberProofTheory.compile_inc_def]
+  fs [clos_numberTheory.compile_inc_def]
   \\ pairarg_tac \\ fs []
   \\ Cases_on `ys` \\ fs [code_locs_def]
   \\ first_x_assum mp_tac
@@ -6765,8 +6759,8 @@ Proof
 QED
 
 Theorem number_oracle_FST_inc:
-  is_state_oracle (ignore_table clos_numberProof$compile_inc) co ==>
-  FST (clos_numberProof$compile_inc (FST (FST (co j))) (FST (SND (co j)))) =
+  is_state_oracle (ignore_table clos_number$compile_inc) co ==>
+  FST (clos_number$compile_inc (FST (FST (co j))) (FST (SND (co j)))) =
     FST (FST (co (j + 1)))
 Proof
   rw [] \\ drule (Q.SPEC `j` backendPropsTheory.is_state_oracle_k)
@@ -6778,14 +6772,14 @@ Proof
 QED
 
 Theorem number_oracle_FST_strict_mono:
-    is_state_oracle (ignore_table clos_numberProof$compile_inc) co ==>
+    is_state_oracle (ignore_table clos_number$compile_inc) co ==>
     !j i. i < j ==> FST (FST (co i)) < FST (FST (co j))
 Proof
   disch_tac \\ Induct \\ fs []
   \\ drule (GEN_ALL number_oracle_FST_inc)
   \\ disch_then (assume_tac o GSYM)
   \\ fs [GSYM arithmeticTheory.ADD1]
-  \\ fs [clos_numberProofTheory.compile_inc_def]
+  \\ fs [clos_numberTheory.compile_inc_def]
   \\ pairarg_tac \\ fs []
   \\ imp_res_tac clos_numberProofTheory.renumber_code_locs_imp_inc
   \\ `FST (FST (co j)) < m` by (
@@ -6802,7 +6796,7 @@ Proof
 QED
 
 Theorem number_oracle_FST_mono:
-    is_state_oracle (ignore_table clos_numberProof$compile_inc) co ==>
+    is_state_oracle (ignore_table clos_number$compile_inc) co ==>
     !j i. i <= j ==> FST (FST (co i)) <= FST (FST (co j))
 Proof
   rw [arithmeticTheory.LESS_OR_EQ]
@@ -6811,11 +6805,11 @@ Proof
 QED
 
 Theorem renumber_code_locs_monotonic:
-    is_state_oracle (ignore_table clos_numberProof$compile_inc) co /\
+    is_state_oracle (ignore_table clos_number$compile_inc) co /\
     FST (FST (co 0)) >= FST (renumber_code_locs_list n exps) ==>
     oracle_monotonic (set ∘ code_locs ∘ FST ∘ SND) $<
         (set (code_locs (SND (renumber_code_locs_list n exps))))
-        (state_co (ignore_table clos_numberProof$compile_inc) co)
+        (state_co (ignore_table clos_number$compile_inc) co)
 Proof
   fs [backendPropsTheory.oracle_monotonic_def, backendPropsTheory.SND_state_co,
     FST_SND_ignore_table]
@@ -6839,7 +6833,7 @@ Theorem SND_cond_mti_compile_inc:
   SND (cond_mti_compile_inc do_it ma v)
     = (if do_it then [] else SND v)
 Proof
-  Cases_on `v` \\ fs [cond_mti_compile_inc_def]
+  Cases_on `v` \\ fs [clos_mtiTheory.cond_mti_compile_inc_def]
     \\ EVERY_CASE_TAC \\ fs [clos_mtiProofTheory.SND_compile_inc]
 QED
 
@@ -6869,9 +6863,9 @@ QED
 
 Theorem number_compile_inc_esgc_free:
   EVERY esgc_free y ==>
-  EVERY esgc_free (SND (clos_numberProof$compile_inc x y))
+  EVERY esgc_free (SND (clos_number$compile_inc x y))
 Proof
-  fs [clos_numberProofTheory.compile_inc_def]
+  fs [clos_numberTheory.compile_inc_def]
   \\ pairarg_tac \\ fs []
   \\ imp_res_tac clos_numberProofTheory.renumber_code_locs_esgc_free
   \\ fs []
@@ -6880,7 +6874,7 @@ QED
 Theorem number_monotonic_elist_globals:
   oracle_monotonic (SET_OF_BAG ∘ elist_globals ∘ FST ∘ SND) $< St co ==>
   oracle_monotonic (SET_OF_BAG ∘ elist_globals ∘ FST ∘ SND) $< St
-       (state_co (ignore_table clos_numberProof$compile_inc) co)
+       (state_co (ignore_table clos_number$compile_inc) co)
 Proof
   match_mp_tac backendPropsTheory.oracle_monotonic_subset
   \\ fs [backendPropsTheory.SND_state_co, FST_SND_ignore_table]
@@ -6894,7 +6888,7 @@ Theorem cond_mti_monotonic_elist_globals:
        (pure_co (cond_mti_compile_inc do_it ma) ∘ co)
 Proof
   match_mp_tac backendPropsTheory.oracle_monotonic_subset
-  \\ fs [cond_mti_compile_inc_def,
+  \\ fs [clos_mtiTheory.cond_mti_compile_inc_def,
     clos_mtiProofTheory.compile_preserves_elist_globals]
   \\ CASE_TAC \\ fs []
   \\ fs [mcompile_inc_uncurry,
@@ -6951,9 +6945,9 @@ Theorem compile_common_semantics:
    (c.do_mti ⇒ 1 ≤ c.max_app ∧ EVERY no_mti es1 ∧
      (∀n. EVERY no_mti (FST(SND(co1 n))))) ∧
    (c.do_call ⇒ every_Fn_vs_NONE es1 /\
-       is_state_oracle clos_callProof$compile_inc
+       is_state_oracle clos_call$compile_inc
            (clos_knownProof$known_co c.known_conf
-               (state_co (ignore_table clos_numberProof$compile_inc)
+               (state_co (ignore_table clos_number$compile_inc)
                    (pure_co (cond_mti_compile_inc c.do_mti c.max_app) ∘ co1)))
            /\
        FST (SND (SND (FST (co1 0)))) = FST (SND (compile c.do_call (SND
@@ -6962,9 +6956,9 @@ Theorem compile_common_semantics:
        1 ≤ c.max_app ∧
        oracle_monotonic (SET_OF_BAG ∘ elist_globals ∘ FST ∘ SND) $<
            (SET_OF_BAG (elist_globals es1)) co1 ∧
-       is_state_oracle (clos_knownProof$compile_inc (THE c.known_conf))
+       is_state_oracle (clos_known$compile_inc (THE c.known_conf))
            (pure_co ^fvs_inc ∘
-               state_co (ignore_table clos_numberProof$compile_inc)
+               state_co (ignore_table clos_number$compile_inc)
                    (pure_co (cond_mti_compile_inc c.do_mti c.max_app) ∘ co1)) /\
        FST (SND (FST (co1 0))) =
            (THE (FST (compile_inc_post_kcompile c es1))).val_approx_spt ∧
@@ -6973,21 +6967,21 @@ Theorem compile_common_semantics:
    ¬contains_App_SOME c.max_app es1 ∧ clos_knownProof$syntax_ok es1 ∧
    (∀n. ¬contains_App_SOME c.max_app (FST(SND(co1 n))) ∧
            every_Fn_vs_NONE (FST (SND (co1 n)))) ∧
-   is_state_oracle (ignore_table clos_numberProof$compile_inc)
+   is_state_oracle (ignore_table clos_number$compile_inc)
        (pure_co (cond_mti_compile_inc c.do_mti c.max_app) ∘ co1) ∧
    FST (FST (co1 0)) >= FST (renumber_code_locs_list (make_even
        (c.next_loc + MAX 1 (LENGTH es1))) (compile c.do_mti c.max_app es1)) ∧
    oracle_monotonic (set ∘ MAP FST ∘ SND ∘ SND) $< (count (FST (FST (co1 0))))
       (state_co (cond_call_compile_inc c.do_call)
          (clos_knownProof$known_co c.known_conf
-            (state_co (ignore_table clos_numberProof$compile_inc)
+            (state_co (ignore_table clos_number$compile_inc)
                (pure_co (cond_mti_compile_inc c.do_mti c.max_app) ∘ co1))))
    ⇒
    closSem$semantics ffi c.max_app (alist_to_fmap code2)
-     (pure_co clos_annotateProof$compile_inc o
+     (pure_co clos_annotate$compile_inc o
        state_co (cond_call_compile_inc c.do_call)
        (clos_knownProof$known_co c.known_conf
-           (state_co (ignore_table clos_numberProof$compile_inc)
+           (state_co (ignore_table clos_number$compile_inc)
              (pure_co (cond_mti_compile_inc c.do_mti c.max_app) o co1))))
      cc ([Call None 0 c'.start []]) =
    closSem$semantics ffi c.max_app FEMPTY co1 (compile_common_inc c cc) es1
@@ -7109,7 +7103,7 @@ Proof
   (* finale *)
   \\ fs []
   \\ Cases_on `c.do_mti`
-  \\ fs [cond_mti_compile_inc_def, clos_mtiTheory.compile_def,
+  \\ fs [clos_mtiTheory.cond_mti_compile_inc_def, clos_mtiTheory.compile_def,
         mcompile_inc_uncurry,
         clos_mtiProofTheory.intro_multi_preserves_elist_globals,
         clos_mtiProofTheory.intro_multi_preserves_esgc_free]
@@ -7198,26 +7192,26 @@ val syntax_oracle_ok_def = Define`
    (c.do_mti ⇒ 1 ≤ c.max_app ∧ EVERY no_mti es ∧
      (∀n. EVERY no_mti (FST(SND(co n))))) ∧
    (?v. FST (co 0) = (c'.next_loc,
-       clos_knownProof$option_val_approx_spt c'.known_conf, FST c'.call_state, v)) ∧
+       clos_known$option_val_approx_spt c'.known_conf, FST c'.call_state, v)) ∧
    (c.do_call ⇒ every_Fn_vs_NONE es ∧
-       is_state_oracle clos_callProof$compile_inc
+       is_state_oracle clos_call$compile_inc
            (clos_knownProof$known_co c.known_conf
-               (state_co (ignore_table clos_numberProof$compile_inc)
+               (state_co (ignore_table clos_number$compile_inc)
                    (pure_co (cond_mti_compile_inc c.do_mti c.max_app) ∘ co)))) ∧
    (IS_SOME c.known_conf ⇒
        1 ≤ c.max_app ∧ every_Fn_vs_NONE es ∧
        oracle_monotonic (SET_OF_BAG ∘ elist_globals ∘ FST ∘ SND) $<
            (SET_OF_BAG (elist_globals es)) co ∧
-       is_state_oracle (clos_knownProof$compile_inc (THE c.known_conf))
+       is_state_oracle (clos_known$compile_inc (THE c.known_conf))
            (pure_co ^fvs_inc ∘
-               state_co (ignore_table clos_numberProof$compile_inc)
+               state_co (ignore_table clos_number$compile_inc)
                    (pure_co (cond_mti_compile_inc c.do_mti c.max_app) ∘ co)) ∧
        (∀n'. BAG_ALL_DISTINCT (elist_globals (FST (SND (co n')))) ∧
                EVERY esgc_free (FST (SND (co n'))))) ∧
    ¬contains_App_SOME c.max_app es ∧ clos_knownProof$syntax_ok es ∧
    (∀n. ¬contains_App_SOME c.max_app (FST(SND(co n))) ∧
            every_Fn_vs_NONE (FST (SND (co n)))) ∧
-   is_state_oracle (ignore_table clos_numberProof$compile_inc)
+   is_state_oracle (ignore_table clos_number$compile_inc)
        (pure_co (cond_mti_compile_inc c.do_mti c.max_app) ∘ co)`;
 
 Theorem compile_exps_IMP_acc:
@@ -7431,14 +7425,14 @@ Theorem annotate_compile_inc_req:
   can_extract (FST prog) ==>
   (ALL_DISTINCT (req_compile_inc_addrs [] prog) ==>
     ALL_DISTINCT (req_compile_inc_addrs []
-        (clos_annotateProof$compile_inc prog)))
+        (clos_annotate$compile_inc prog)))
     /\
-  can_extract (FST (clos_annotateProof$compile_inc prog)) /\
-  set (req_compile_inc_addrs [] (clos_annotateProof$compile_inc prog)) ⊆
+  can_extract (FST (clos_annotate$compile_inc prog)) /\
+  set (req_compile_inc_addrs [] (clos_annotate$compile_inc prog)) ⊆
     set (req_compile_inc_addrs [] prog)
 Proof
   PairCases_on `prog`
-  \\ fs [clos_annotateProofTheory.compile_inc_def, req_compile_inc_addrs_def]
+  \\ fs [clos_annotateTheory.compile_inc_def, req_compile_inc_addrs_def]
   \\ disch_tac
   \\ drule_then assume_tac can_extract_to_case \\ fs []
   \\ fs [annotate_Op_Const, EVAL ``annotate arity []``, show_SUBSET]
@@ -7461,7 +7455,7 @@ val annotate_compile_inc_req_intros = UNDISCH_ALL annotate_compile_inc_req
   |> CONJUNCTS |> map (IRULE_CANON o DISCH_ALL)
 
 val annotate_compile_inc_req_oracle = mk_to_oracle
-  ``\orac1. pure_co clos_annotateProof$compile_inc o orac1`` `[]`
+  ``\orac1. pure_co clos_annotate$compile_inc o orac1`` `[]`
 
 Theorem annotate_compile_every_Fn_vs_SOME:
   every_Fn_vs_SOME (MAP (SND o SND) (clos_annotate$compile es))
@@ -7482,7 +7476,7 @@ Theorem cond_call_compile_inc_req:
     set (req_compile_inc_addrs [SUC] prog)
 Proof
   PairCases_on `prog`
-  \\ fs [cond_call_compile_inc_def, req_compile_inc_addrs_def]
+  \\ fs [clos_callTheory.cond_call_compile_inc_def, req_compile_inc_addrs_def]
   \\ reverse CASE_TAC
   >- (
     fs [req_compile_inc_addrs_def, code_locs_def, show_SUBSET]
@@ -7573,16 +7567,16 @@ Theorem known_co_req:
 Proof
   fs [clos_knownProofTheory.known_co_def]
   \\ CASE_TAC \\ fs [backendPropsTheory.SND_state_co]
-  \\ qmatch_goalsub_abbrev_tac `clos_knownProof$compile_inc _ _ prog1`
-  \\ qmatch_goalsub_abbrev_tac `clos_ticksProof$compile_inc prog2`
-  \\ qmatch_goalsub_abbrev_tac `clos_letopProof$compile_inc prog3`
+  \\ qmatch_goalsub_abbrev_tac `clos_known$compile_inc _ _ prog1`
+  \\ qmatch_goalsub_abbrev_tac `clos_ticks$compile_inc prog2`
+  \\ qmatch_goalsub_abbrev_tac `clos_letop$compile_inc prog3`
   \\ qmatch_goalsub_abbrev_tac `set (req_compile_inc_addrs _ prog4) ⊆ _`
   \\ qho_match_abbrev_tac `P (SND (orac n)) prog4`
   \\ `P prog3 prog4 /\ P (SND (orac n)) prog3` suffices_by
     (unabbrev_all_tac \\ metis_tac [SUBSET_TRANS])
   \\ conj_tac >- (
     Cases_on `prog3` \\ qunabbrev_tac `prog4` \\ qunabbrev_tac `P`
-    \\ fs [clos_letopProofTheory.compile_inc_def]
+    \\ fs [clos_letopTheory.compile_inc_def]
     \\ disch_tac \\ fs []
     \\ drule_then assume_tac can_extract_to_case \\ fs []
     \\ fs [let_op_Op_Const] \\ fs [clos_letopTheory.let_op_def]
@@ -7597,7 +7591,7 @@ Proof
     (unabbrev_all_tac \\ metis_tac [SUBSET_TRANS])
   \\ conj_tac >- (
     Cases_on `prog2` \\ qunabbrev_tac `prog3` \\ qunabbrev_tac `P`
-    \\ fs [clos_ticksProofTheory.compile_inc_def]
+    \\ fs [clos_ticksTheory.compile_inc_def]
     \\ disch_tac \\ fs []
     \\ drule_then assume_tac can_extract_to_case \\ fs []
     \\ fs [clos_ticksTheory.remove_ticks_def, can_extract_def]
@@ -7658,13 +7652,13 @@ val known_co_req_oracle = mk_to_oracle
     ``\orac. clos_knownProof$known_co kc orac`` `[SUC]`
 
 Theorem number_compile_inc_req:
-  let nprog = SND (ignore_table clos_numberProof$compile_inc n prog) in
+  let nprog = SND (ignore_table clos_number$compile_inc n prog) in
   SND prog = [] ==>
   ALL_DISTINCT (req_compile_inc_addrs [SUC] nprog) /\
   SND nprog = [] /\ can_extract (FST nprog)
 Proof
   PairCases_on `prog` \\ fs [ignore_table_def]
-  \\ fs [clos_numberProofTheory.compile_inc_def]
+  \\ fs [clos_numberTheory.compile_inc_def]
   \\ rpt (pairarg_tac \\ fs [])
   \\ rpt disch_tac
   \\ rveq \\ fs []
@@ -7698,12 +7692,12 @@ val number_compile_inc_req_intros = number_compile_inc_req
 
 Theorem MEM_number_req:
   MEM x (req_compile_inc_addrs [SUC]
-    (SND (ignore_table clos_numberProof$compile_inc n prog))) /\
+    (SND (ignore_table clos_number$compile_inc n prog))) /\
   SND prog = [] ==>
-  n <= x /\ x < FST (clos_numberProof$compile_inc n (FST prog))
+  n <= x /\ x < FST (clos_number$compile_inc n (FST prog))
 Proof
   PairCases_on `prog` \\ Cases_on `prog1` \\ fs [ignore_table_def]
-  \\ fs [clos_numberProofTheory.compile_inc_def]
+  \\ fs [clos_numberTheory.compile_inc_def]
   \\ specl_args_of_then``renumber_code_locs_list``
         clos_numberProofTheory.renumber_code_locs_list_distinct mp_tac
   \\ specl_args_of_then ``renumber_code_locs_list``
@@ -7729,11 +7723,11 @@ Proof
 QED
 
 Theorem renumber_code_locs_monotonic_req:
-    is_state_oracle (ignore_table clos_numberProof$compile_inc) co /\
+    is_state_oracle (ignore_table clos_number$compile_inc) co /\
     (!x. x ∈ St ==> FST (FST (co 0)) + offs > x) /\
     (!n. SND (SND (co n)) = []) ==>
     oracle_monotonic (set ∘ MAP ($+ offs) ∘ req_compile_inc_addrs [SUC] ∘ SND)
-        $< St (state_co (ignore_table clos_numberProof$compile_inc) co)
+        $< St (state_co (ignore_table clos_number$compile_inc) co)
 Proof
   fs [backendPropsTheory.oracle_monotonic_def, backendPropsTheory.SND_state_co,
     FST_SND_ignore_table, MEM_MAP]
@@ -7795,7 +7789,7 @@ QED
 Theorem LENGTH_FST_cond_mti_compile_inc:
   LENGTH (FST (cond_mti_compile_inc do_it ma prog)) = LENGTH (FST prog)
 Proof
-  fs [cond_mti_compile_inc_def]
+  fs [clos_mtiTheory.cond_mti_compile_inc_def]
   \\ CASE_TAC \\ fs []
   \\ fs [mcompile_inc_uncurry, clos_mtiTheory.intro_multi_length]
 QED
@@ -7804,7 +7798,7 @@ Theorem every_Fn_vs_NONE_cond_mti_compile_inc:
   every_Fn_vs_NONE (FST (cond_mti_compile_inc do_it ma prog)) =
     every_Fn_vs_NONE (FST prog)
 Proof
-  fs [cond_mti_compile_inc_def]
+  fs [clos_mtiTheory.cond_mti_compile_inc_def]
   \\ CASE_TAC \\ fs []
   \\ fs [mcompile_inc_uncurry]
 QED
@@ -7905,15 +7899,15 @@ fun abbrev_adj_tac f = first_assum (fn t => if not
     val (v_nm, _) = dest_var v
     val x = f rhs
     val v2 = mk_var (v_nm ^ "'", type_of x)
-  in markerLib.ABBREV_TAC (mk_eq (v2, x)) \\ markerLib.UNABBREV_TAC v_nm end)
+  in markerLib.ABBREV_TAC (mk_eq (v2, x)) \\ markerLib.UNABBREV_TAC v_nm end);
 
 Theorem syntax_oracle_ok_to_oracle_inv:
   ∀cc es co c c'. syntax_oracle_ok c c' es co /\
     compile_common c es = (c', prog') ==>
-  let co' = pure_co clos_annotateProof$compile_inc ∘
+  let co' = pure_co clos_annotate$compile_inc ∘
         state_co (cond_call_compile_inc c.do_call)
           (clos_knownProof$known_co c.known_conf
-             (state_co (ignore_table clos_numberProof$compile_inc)
+             (state_co (ignore_table clos_number$compile_inc)
                 (pure_co (cond_mti_compile_inc c.do_mti c.max_app) ∘ co))) in
   compile_oracle_inv c.max_app (alist_to_fmap prog')
     (pure_cc (compile_inc c.max_app) cc) co'
@@ -7994,7 +7988,7 @@ Proof
   \\ TRY (imp_res_tac clos_knownProofTheory.known_compile_IS_SOME)
   \\ fs []
   \\ fs [num_stubs_def, IS_SOME_EXISTS,
-        clos_knownProofTheory.option_val_approx_spt_def]
+        clos_knownTheory.option_val_approx_spt_def]
 QED
 
 Theorem compile_every_Fn_SOME:
@@ -8181,8 +8175,8 @@ Proof
 QED
 
 Theorem mcompile_inc_nil:
-   (FST p = [] ⇒ (clos_mtiProof$compile_inc max_app p = ([],[]))) ∧
-   (FST p ≠ [] ⇒ FST (clos_mtiProof$compile_inc max_app p) ≠ [])
+   (FST p = [] ⇒ (clos_mti$compile_inc max_app p = ([],[]))) ∧
+   (FST p ≠ [] ⇒ FST (clos_mti$compile_inc max_app p) ≠ [])
 Proof
   Cases_on`p` \\ rw[] \\ EVAL_TAC
   \\ strip_tac \\ fs[]
@@ -8282,7 +8276,7 @@ Theorem syntax_oracle_ok_call_FST_monotonic:
   oracle_monotonic (set ∘ MAP FST ∘ SND ∘ SND) $< (count (FST (FST (co 0))))
      (state_co (cond_call_compile_inc c.do_call)
         (clos_knownProof$known_co c.known_conf
-           (state_co (ignore_table clos_numberProof$compile_inc)
+           (state_co (ignore_table clos_number$compile_inc)
               (pure_co (cond_mti_compile_inc c.do_mti c.max_app) ∘ co))))
 Proof
   rw [] \\ fs [syntax_oracle_ok_def]
@@ -8324,10 +8318,10 @@ Theorem compile_semantics:
    ⇒
    semantics ffi (fromAList prog)
      (pure_co (compile_inc c.max_app) o
-      pure_co clos_annotateProof$compile_inc o
+      pure_co clos_annotate$compile_inc o
       state_co (cond_call_compile_inc c.do_call)
         (clos_knownProof$known_co c.known_conf
-          (state_co (ignore_table clos_numberProof$compile_inc)
+          (state_co (ignore_table clos_number$compile_inc)
             (pure_co (cond_mti_compile_inc c.do_mti c.max_app) ∘ co))))
        cc c'.start =
    semantics ffi c.max_app FEMPTY co
@@ -8351,7 +8345,7 @@ Proof
     \\ fs [compile_inc_post_kcompile_def]
     \\ imp_res_tac clos_knownProofTheory.known_compile_IS_SOME
     \\ rw [IS_SOME_EXISTS]
-    \\ fs [clos_knownProofTheory.option_val_approx_spt_def, IS_SOME_EXISTS]
+    \\ fs [clos_knownTheory.option_val_approx_spt_def, IS_SOME_EXISTS]
   )
   \\ disch_then(assume_tac o SYM) \\ fs[]
   \\ irule compile_prog_semantics
@@ -8454,11 +8448,11 @@ Proof
 
 Theorem compile_inc_phases_all_distinct:
   SND (SND (orac i)) = [] ==>
-  ALL_DISTINCT (MAP FST (clos_to_bvlProof$compile_inc max_app
-    (clos_annotateProof$compile_inc
-      (SND (clos_to_bvlProof$cond_call_compile_inc dc c_st
+  ALL_DISTINCT (MAP FST (clos_to_bvl$compile_inc max_app
+    (clos_annotate$compile_inc
+      (SND (clos_call$cond_call_compile_inc dc c_st
         (SND (clos_knownProof$known_co kc
-          (state_co (closProps$ignore_table clos_numberProof$compile_inc) orac)
+          (state_co (closProps$ignore_table clos_number$compile_inc) orac)
             i)))))))
 Proof
   rw []
@@ -8477,10 +8471,10 @@ Theorem syntax_oracle_ok_bvl_FST_monotonic:
   oracle_monotonic (set ∘ MAP FST ∘ SND) $<
      (count (FST (FST (co 0)) + num_stubs c.max_app))
      (pure_co (compile_inc c.max_app) o
-      pure_co clos_annotateProof$compile_inc o
+      pure_co clos_annotate$compile_inc o
       (state_co (cond_call_compile_inc c.do_call)
         (clos_knownProof$known_co c.known_conf
-           (state_co (ignore_table clos_numberProof$compile_inc)
+           (state_co (ignore_table clos_number$compile_inc)
               (pure_co (cond_mti_compile_inc c.do_mti c.max_app) ∘ co)))))
 Proof
   simp [clos_to_bvlTheory.compile_def]
